other tests of spec monad

iodiv/DivFreeTauSpec.Test.fst
@@ -1,13 +1,56 @@
 module DivFreeTauSpec.Test
 
+open FStar.Tactics
+
 open DivFreeTauSpec
+open IIOSigSpec
 
+(** 
+let dm sg (w_act : action_iwp sg) (a : Type) (w : iwp a) =
+  c : m sg a { theta w_act c `ile` w }
 
-let test1 : iwp unit =
+**)
+
+let triv #a : iwp a =
+  iprepost (fun _ -> True) (fun h r -> True) 
+
+let r_div : iwp unit =
   iprepost (fun _ -> True) (fun h r -> diverges r)
 
-let testfalse : iwp unit =
+let r_cv : iwp unit =
+  iprepost (fun _ -> True) (fun h r -> terminates r)
+
+(** *** Append assert false to divergent code **)
+
+let assert_false : iwp unit =
   iprepost (fun _ -> False) (fun h r -> True)
 
-// TODO: is this surprising?
-let d = assert (test1 `ile` i_bind test1 (fun _ -> testfalse))
+let _ = assert (i_bind r_div (fun _ -> assert_false) `ile` r_div)
+(** This is not surprising taking in consideration the definition of `i_bind`.
+   If we unfold it, we obtain something similar to:
+   (fun post hist ->
+      w (fun r ->
+        match r with
+        | Cv tr x -> wf x (ishift_post tr post) (rev_acc (to_trace tr) hist)
+        | Dv st -> post (Dv st)
+        ) hist)
+
+   and here one can see that `wf` (which is `(fun _ -> testfalse)` in our case)
+   is not used in the `Dv` branch.
+
+   TODO: is this a problem?
+**)
+
+
+[@expect_failure] (** fails goal 2 that requires to prove False **)
+let _ = assert (i_bind r_cv (fun _ -> assert_false) `ile` r_cv) by (norm [delta_only [`%r_cv;`%iprepost]]; explode ();dump "H")
+
+
+(** *** Actions **)
+
+let _ = assert (i_open "test.txt" `ile` triv)
+let _ = assert (i_bind (i_open "test.txt") (fun _ -> i_ret ()) `ile` triv)
+let _ = assert (i_bind (i_open "test.txt") (fun _ -> i_ret ()) `ile` r_cv)
+  
+[@expect_failure]
+let _ = assert (i_bind (i_open "test.txt") (fun _ -> i_ret ()) `ile` r_div) by (norm [delta_only [`%r_div;`%iprepost;`%i_ret;`%ishift_post;`%as_iwp;`%ishift_post;`%ret_fin_trace];zeta]; explode (); bump_nth 2; compute ();explode (); dump "H")
